x+ay+m = 2(x+by+m)
x+m=(a-2b)y

/**
 * Definition for singly-linked list.
 * class ListNode {
 *     int val;
 *     ListNode next;
 *     ListNode(int x) {
 *         val = x;
 *         next = null;
 *     }
 * }
 */
public class Solution {
    public ListNode detectCycle(ListNode head) {
        ListNode fast = head;
        ListNode slow = head;
        do{
            if(fast != null)
                fast = fast.next;
            else
                return null;
            if(fast != null)
                fast = fast.next;
            else
                return null;
            slow = slow.next;
        }while(fast != slow);
        fast = head;
        
        while(fast != slow){
            fast = fast.next;
            slow = slow.next;
        }
        return slow;
    }
} 
